coq/cclc/clc_eval.v
@@ -1,0 +1,118 @@
+From mathcomp Require Import ssreflect ssrbool eqtype ssrnat seq.
+From Coq Require Import ssrfun Utf8 Classical.
+Require Import AutosubstSsr ARS 
+  clc_context clc_ast clc_confluence clc_subtype clc_typing
+  clc_weakening clc_substitution clc_inversion clc_validity
+  clc_soundness.
+
+Definition env T := seq (nat * T).
+
+Fixpoint free0 {T} (e : env T) (l : nat) : env T :=
+  match e with
+  | nil => nil
+  | (addr, m) :: e =>
+    if l == addr then e else (addr, m) :: free0 e l
+  end.
+
+Definition free {T} (e : env T) (l : nat) (t : sort) := 
+  match t with
+  | U => e
+  | L => free0 e l
+  end.
+
+Inductive open {T} : env T -> nat -> Prop :=
+| open_nil l : 
+  open nil l
+| open_cons e l addr m :
+  open e l ->
+  l <> addr ->
+  open ((addr, m) :: e) l.
+
+Inductive mapsto {T} : env T -> nat -> T -> Prop :=
+| mapsto0 e l m :
+  mapsto ((l, m) :: e) l m
+| mapsto1 e l addr m n :
+  mapsto e l m ->
+  mapsto ((addr, n) :: e) l m.
+
+Inductive eterm :=
+| eVar    (x : var)
+| eLab    (l : nat)
+| eSort   (s : sort) (l : nat)
+| ePi     (A : eterm) (B : {bind eterm}) (s t : sort)
+| eLam    (A : eterm) (B : {bind eterm}) (s t : sort)
+| eApp    (m n : eterm)
+| eUnit
+| eIt
+| eSigma  (A : eterm) (B : {bind eterm}) (s r t : sort)
+| ePair   (m n : eterm)
+| eLetIn1 (m n : eterm)
+| eLetIn2 (m n : eterm).
+
+Instance Ids_eterm : Ids eterm. derive. Defined.
+Instance Rename_eterm : Rename eterm. derive. Defined.
+Instance Subst_eterm : Subst eterm. derive. Defined.
+Instance substLemmas_eterm : SubstLemmas eterm. derive. Qed.
+
+Fixpoint embed (tm : term) : eterm :=
+  match tm with
+  | Var x => eVar x
+  | Sort s l => eSort s l
+  | Pi A B s t => ePi (embed A) (embed B) s t
+  | Lam A m s t => eLam (embed A) (embed m) s t
+  | App m n => eApp (embed m) (embed n)
+  | Unit => eUnit
+  | It => eIt
+  | Sigma A B s r t => eSigma (embed A) (embed B) s r t
+  | Pair m n => ePair (embed m) (embed n)
+  | LetIn1 m n => eLetIn1 (embed m) (embed n)
+  | LetIn2 m n => eLetIn2 (embed m) (embed n)
+  end.
+Notation "[[ m ]]" := (embed m).
+
+Reserved Notation "Θ ;; m => Θ' ;; n" 
+  (at level 80, m, Θ', n at next level).
+
+Inductive eval : env eterm -> eterm -> env eterm -> eterm -> Prop :=
+| eval_sort Θ s i l :
+  open Θ l ->
+  Θ ;; eSort s i => (l, eSort s i) :: Θ ;; eLab l
+| eval_pi Θ A B s t l :
+  open Θ l ->
+  Θ ;; ePi A B s t => (l, ePi A B s t) :: Θ ;; eLab l
+| eval_lam Θ A m s t l :
+  open Θ l ->
+  Θ ;; eLam A m s t => (l, eLam A m s t) :: Θ ;; eLab l
+| eval_appL Θ Θ' m m' n :
+  Θ ;; m => Θ' ;; m' ->
+  Θ ;; eApp m n => Θ' ;; eApp m' n
+| eval_appR Θ Θ' l n n' :
+  Θ ;; n => Θ' ;; n' ->
+  Θ ;; eApp (eLab l) n => Θ' ;; eApp (eLab l) n'
+| eval_beta Θ Θ' lf la A m s t :
+  Θ' = free Θ lf t ->
+  mapsto Θ lf (eLam A m s t) ->
+  Θ ;; eApp (eLab lf) (eLab la) => Θ' ;; m.[eLab la/]
+| eval_unit Θ l :
+  open Θ l ->
+  Θ ;; eUnit => (l, eUnit) :: Θ ;; eLab l
+| eval_it Θ l :
+  open Θ l ->
+  Θ ;; eIt => (l, eIt) :: Θ ;; eLab l
+| eval_sigma Θ A B s r t l :
+  open Θ l ->
+  Θ ;; eSigma A B s r t => (l, eSigma A B s r t) :: Θ ;; eLab l
+| eval_pairL Θ Θ' m m' n :
+  Θ ;; m => Θ' ;; m' ->
+  Θ ;; ePair m n => Θ' ;; ePair m' n
+| eval_pairR Θ Θ' l n n' :
+  Θ ;; n => Θ' ;; n' ->
+  Θ ;; ePair (eLab l) n => Θ' ;; ePair (eLab l) n'
+| eval_letin1 Θ Θ' m m' n :
+  Θ ;; m => Θ' ;; m' ->
+  Θ ;; eLetIn1 m n => Θ' ;; eLetIn1 m' n
+| eval_iota1 Θ l n :
+  mapsto Θ l eIt ->
+  Θ ;; eLetIn1 (eLab l) n => Θ ;; n
+
+where "Θ ;; m => Θ' ;; n" := (eval Θ m Θ' n).
